theory/bpfConsistencyAux.thy
@@ -13,16 +13,16 @@ u8_of_ireg ri = ucast(bpf_ireg2u4 src) \<Longrightarrow>*)
 lemma addl_subgoal_rr:
       "bins = BPF_ALU BPF_ADD dst (SOReg src) \<Longrightarrow>
        xins = Paddl_rr rd ri \<Longrightarrow>
-       (BPF_OK rs' m' ss'  is_v1 cur_cu remain_cu) = step bins rs m ss is_v1 cur_cu remain_cu \<Longrightarrow>
+       (BPF_OK pc rs' m' ss' is_v1 (cur_cu+1) remain_cu) = step fuel bins rs m ss is_v1 cur_cu remain_cu \<Longrightarrow>
        Next reg' m'  = exec_instr xins sz reg m \<Longrightarrow> 
-       corr_registers dst rd \<Longrightarrow>
-       corr_registers src ri \<Longrightarrow>
+       rd = bpf_to_x64_reg dst \<Longrightarrow>
+       ri = bpf_to_x64_reg src \<Longrightarrow>
        reg (IR rd) = Vint n1 \<Longrightarrow>
        reg (IR ri) = Vint n2 \<Longrightarrow>
-       ucast n1 = rs (BR dst) \<Longrightarrow>
-       ucast n2  = rs (BR src) \<Longrightarrow>
+       ucast n1 = rs dst \<Longrightarrow>
+       ucast n2  = rs src \<Longrightarrow>
        reg' (IR rd) = Vint n3 \<Longrightarrow>
-       ucast n3 = rs'(BR dst)"
+       ucast n3 = rs'dst"
   apply (unfold exec_instr_def step)
   apply simp
   apply (unfold eval_alu32_def)
@@ -42,14 +42,14 @@ lemma addl_subgoal_rr:
 lemma addl_subgoal_ri:
       "bins = BPF_ALU BPF_ADD dst (SOImm src) \<Longrightarrow>
        xins = Paddl_ri rd imm \<Longrightarrow>
-       (BPF_OK rs' m' ss'  is_v1 cur_cu remain_cu) = step bins rs m ss is_v1 cur_cu remain_cu \<Longrightarrow>
-       Next reg' m'  = exec_instr xins sz reg m \<Longrightarrow> 
-       corr_registers dst rd \<Longrightarrow>
+       (BPF_OK pc rs' m' ss' is_v1 (cur_cu+1) remain_cu) = step fuel bins rs m ss is_v1 cur_cu remain_cu \<Longrightarrow>
+       Next reg' m' = exec_instr xins sz reg m \<Longrightarrow> 
+       rd = bpf_to_x64_reg dst \<Longrightarrow>
        imm = ucast (src) \<Longrightarrow>
        reg (IR rd) = Vint n1 \<Longrightarrow>
-       ucast n1  = rs (BR dst) \<Longrightarrow>
+       ucast n1  = rs dst \<Longrightarrow>
        reg' (IR rd) = Vint n3 \<Longrightarrow>
-       ucast n3 = rs'(BR dst)"
+       ucast n3 = rs'dst"
   apply (unfold exec_instr_def step)
   apply simp
   apply (unfold eval_alu32_def)
@@ -69,16 +69,16 @@ lemma addl_subgoal_ri:
 lemma addq_subgoal_rr:
       "bins = BPF_ALU64 BPF_ADD dst (SOReg src) \<Longrightarrow>
        xins = Paddq_rr rd ri \<Longrightarrow>
-       (BPF_OK rs' m' ss'  is_v1 cur_cu remain_cu) = step  bins rs m ss is_v1 cur_cu remain_cu \<Longrightarrow>
+       (BPF_OK pc rs' m' ss' is_v1 (cur_cu+1) remain_cu) = step fuel bins rs m ss is_v1 cur_cu remain_cu \<Longrightarrow>
        Next reg' m'  = exec_instr xins sz reg m \<Longrightarrow> 
        corr_registers dst rd \<Longrightarrow>
        corr_registers src ri \<Longrightarrow>
        reg (IR rd) = Vlong n1 \<Longrightarrow>
        reg (IR ri) = Vlong n2 \<Longrightarrow>
-       n1  = rs (BR dst) \<Longrightarrow>
-       n2  = rs (BR src) \<Longrightarrow>
+       n1  = rs dst \<Longrightarrow>
+       n2  = rs src \<Longrightarrow>
        reg' (IR rd) = Vlong n3 \<Longrightarrow>
-       ucast n3 = rs'(BR dst)"
+       ucast n3 = rs'dst"
   apply (unfold exec_instr_def step)
   apply simp
   apply (unfold eval_alu64_def)
@@ -156,35 +156,35 @@ lemma load_subgoal_aux1:
        ri = (bpf_to_x64_reg src) \<Longrightarrow>
        reg (IR rd) = Vlong n1 \<Longrightarrow>
        reg (IR ri) = Vlong n2 \<Longrightarrow>
-       n1  = rs (BR dst) \<Longrightarrow>
-       n2  = rs (BR src) \<Longrightarrow>
-       (BPF_OK rs' mem' ss'  is_v1 cur_cu remain_cu) = step  bins rs mem ss is_v1 cur_cu remain_cu \<Longrightarrow>
+       n1  = rs dst \<Longrightarrow>
+       n2  = rs src \<Longrightarrow>
+       (BPF_OK pc rs' mem' ss' is_v1 cur_cu remain_cu) = step fuel bins rs mem ss is_v1 cur_cu remain_cu \<Longrightarrow>
        Next reg' m'  = exec_instr xins sz reg m \<Longrightarrow> 
        m = mem \<Longrightarrow>
        m' = mem'"
   apply (unfold exec_instr_def step)
   apply(cases xins)
   apply simp_all
-  apply (unfold eval_load_def Let_def cast_lemma5, simp_all)
+  apply (unfold eval_load_def Let_def cast_lemma6, simp_all)
   apply (simp add: exec_load_def eval_addrmode64_def add64_def nextinstr_nf_def nextinstr_def)
   by (metis (mono_tags, lifting) bpf_state.distinct(1) bpf_state.inject option.case_eq_if outcome.distinct(1) outcome.inject)
 
 lemma load_subgoal_aux2_1:
   assumes a0:"bins = BPF_LDX chk dst src b_off" and 
-          a1:"step bins rs mem ss is_v1 cur_cu remain_cu = result"
-        shows "result = (BPF_OK rs' mem' ss'  is_v1 cur_cu remain_cu) \<longrightarrow> Mem.loadv chk mem (Vlong (eval_snd_op_u64 (SOReg src) rs + scast b_off)) \<noteq> Some Vundef"
+          a1:"step fuel bins rs mem ss is_v1 cur_cu remain_cu = result"
+        shows "result = (BPF_OK pc rs' mem' ss' is_v1 (cur_cu+1) remain_cu) \<longrightarrow> Mem.loadv chk mem (Vlong (eval_snd_op_u64 (SOReg src) rs + scast b_off)) \<noteq> Some Vundef"
 proof (rule ccontr)
-  assume a2:"\<not> (result = (BPF_OK rs' mem' ss'  is_v1 cur_cu remain_cu) \<longrightarrow> (Mem.loadv chk mem (Vlong (eval_snd_op_u64 (SOReg src) rs + scast b_off)) \<noteq> Some Vundef))"
+  assume a2:"\<not> (result = (BPF_OK pc rs' mem' ss' is_v1 (cur_cu+1) remain_cu) \<longrightarrow> (Mem.loadv chk mem (Vlong (eval_snd_op_u64 (SOReg src) rs + scast b_off)) \<noteq> Some Vundef))"
   let ?x = "eval_snd_op_u64 (SOReg src) rs + scast b_off"
   let ?tmp = "Mem.loadv chk mem (Vlong ?x)"
-  let ?res_ok = "(BPF_OK rs' mem' ss'  is_v1 cur_cu remain_cu)"
+  let ?res_ok = "(BPF_OK pc rs' mem' ss' is_v1 (cur_cu+1) remain_cu)"
   have a3:"\<not> (\<not> result = ?res_ok \<or> (?tmp \<noteq> Some Vundef))" using imp_conv_disj a2 by blast
   have a4:"result = ?res_ok \<and> ?tmp = Some Vundef" using a3 by simp
    then show "False"
    proof
      have b0:"?tmp = Some Vundef" using a4 conjE by simp
      have b1:"eval_load chk dst src b_off rs mem = None"  using eval_load_def b0 by simp
-     have b2: "step bins rs mem ss is_v1 cur_cu remain_cu = BPF_EFlag"using a0 b1 eval_load_def by simp
+     have b2: "step fuel bins rs mem ss is_v1 cur_cu remain_cu = BPF_EFlag"using a0 b1 eval_load_def by simp
      thus "False" using b2 
        by (metis a1 a4 bpf_state.distinct(3))
    qed
@@ -192,20 +192,20 @@ proof (rule ccontr)
 
 lemma load_subgoal_aux2_2:
   assumes a0:"bins = BPF_LDX chk dst src b_off" and 
-          a1:"step  bins rs mem ss is_v1 cur_cu remain_cu = result"
-        shows "result = (BPF_OK rs' mem' ss'  is_v1 cur_cu remain_cu) \<longrightarrow> Mem.loadv chk mem (Vlong (eval_snd_op_u64 (SOReg src) rs + scast b_off)) \<noteq> None"
+          a1:"step fuel bins rs mem ss is_v1 cur_cu remain_cu = result"
+        shows "result = (BPF_OK pc rs' mem' ss' is_v1 (cur_cu+1) remain_cu) \<longrightarrow> Mem.loadv chk mem (Vlong (eval_snd_op_u64 (SOReg src) rs + scast b_off)) \<noteq> None"
 proof (rule ccontr)
-  assume a2:"\<not> (result = (BPF_OK rs' mem' ss'  is_v1 cur_cu remain_cu) \<longrightarrow> (Mem.loadv chk mem (Vlong (eval_snd_op_u64 (SOReg src) rs + scast b_off)) \<noteq> None))"
+  assume a2:"\<not> (result = (BPF_OK pc rs' mem' ss' is_v1 (cur_cu+1) remain_cu) \<longrightarrow> (Mem.loadv chk mem (Vlong (eval_snd_op_u64 (SOReg src) rs + scast b_off)) \<noteq> None))"
   let ?x = "eval_snd_op_u64 (SOReg src) rs + scast b_off"
   let ?tmp = "Mem.loadv chk mem (Vlong ?x)"
-  let ?res_ok = "(BPF_OK rs' mem' ss'  is_v1 cur_cu remain_cu)"
+  let ?res_ok = "(BPF_OK pc rs' mem' ss' is_v1 (cur_cu+1) remain_cu)"
   have a3:"\<not> (\<not> result = ?res_ok \<or> (?tmp \<noteq> None))" using imp_conv_disj a2 by blast
   have a4:"result = ?res_ok \<and> ?tmp = None" using a3 by simp
    then show "False"
    proof
      have b0:"?tmp = None" using a4 conjE by simp
      have b1:"eval_load chk dst src b_off rs mem = None"  using eval_load_def b0 by simp
-     have b2: "step  bins rs mem ss is_v1 cur_cu remain_cu = BPF_EFlag"using a0 b1 eval_load_def by simp
+     have b2: "step fuel bins rs mem ss is_v1 cur_cu remain_cu = BPF_EFlag"using a0 b1 eval_load_def by simp
      thus "False" using b2 
        using a1 a4 by auto
    qed
@@ -213,23 +213,23 @@ proof (rule ccontr)
 
 lemma load_subgoal_aux2_3:
   assumes a0:"bins = BPF_LDX chk dst src b_off" and 
-          a1:"step  bins rs mem ss is_v1 cur_cu remain_cu = result"
-        shows "result = (BPF_OK rs' mem' ss'  is_v1 cur_cu remain_cu) \<longrightarrow> Mem.loadv chk mem (Vlong (eval_snd_op_u64 (SOReg src) rs + scast b_off)) \<notin> {None, Some Vundef} "
+          a1:"step fuel bins rs mem ss is_v1 cur_cu remain_cu = result"
+        shows "result = (BPF_OK pc rs' mem' ss' is_v1 (cur_cu+1) remain_cu) \<longrightarrow> Mem.loadv chk mem (Vlong (eval_snd_op_u64 (SOReg src) rs + scast b_off)) \<notin> {None, Some Vundef} "
   using load_subgoal_aux2_1 load_subgoal_aux2_2 a0 a1 by auto
 
 lemma load_subgoal_aux2_4:
   assumes a0:"bins = BPF_LDX chk dst src b_off" and 
-          a1:"step  bins rs mem ss is_v1 cur_cu remain_cu = result"
-        shows "result = (BPF_OK rs' mem' ss'  is_v1 cur_cu remain_cu) \<longrightarrow> eval_load chk dst src b_off rs mem \<noteq> None"
+          a1:"step fuel bins rs mem ss is_v1 cur_cu remain_cu = result"
+        shows "result = (BPF_OK pc rs' mem' ss' is_v1 (cur_cu+1) remain_cu) \<longrightarrow> eval_load chk dst src b_off rs mem \<noteq> None"
 proof (rule ccontr)
-  assume a2:"\<not> (result = (BPF_OK rs' mem' ss'  is_v1 cur_cu remain_cu) \<longrightarrow> eval_load chk dst src b_off rs mem \<noteq> None)"
-  let ?res_ok = "(BPF_OK rs' mem' ss'  is_v1 cur_cu remain_cu)"
+  assume a2:"\<not> (result = (BPF_OK pc rs' mem' ss' is_v1 (cur_cu+1) remain_cu) \<longrightarrow> eval_load chk dst src b_off rs mem \<noteq> None)"
+  let ?res_ok = "(BPF_OK pc rs' mem' ss' is_v1 (cur_cu+1) remain_cu)"
   have a3:"\<not> (\<not> result = ?res_ok \<or> (eval_load chk dst src b_off rs mem \<noteq> None))" using imp_conv_disj a2 by blast
   have a4:"result = ?res_ok \<and> (eval_load chk dst src b_off rs mem = None)" using a3 by simp
    then show "False"
    proof
      have b1:"eval_load chk dst src b_off rs mem = None" using a4 conjE by simp
-     have b2: "step  bins rs mem ss is_v1 cur_cu remain_cu = BPF_EFlag"using a0 b1 eval_load_def by simp
+     have b2: "step fuel bins rs mem ss is_v1 cur_cu remain_cu = BPF_EFlag"using a0 b1 eval_load_def by simp
      thus "False" using b2 a1 a0 a2 by auto
    qed
  qed
@@ -241,24 +241,24 @@ proof (rule ccontr)
        ri = (bpf_to_x64_reg src) \<Longrightarrow>
        reg (IR rd) = Vlong n1 \<Longrightarrow>
        reg (IR ri) = Vlong n2 \<Longrightarrow>
-       n1  = rs (BR dst) \<Longrightarrow>
-       n2  = rs (BR src) \<Longrightarrow>
+       n1  = rs dst \<Longrightarrow>
+       n2  = rs src \<Longrightarrow>
        b_off = scast x_off \<Longrightarrow>
        (BPF_OK rs' mem' ss'  is_v1 cur_cu remain_cu) = step  bins rs mem ss is_v1 cur_cu remain_cu \<Longrightarrow>
        Next reg' m'  = exec_instr xins sz reg m \<Longrightarrow> 
        m = mem \<Longrightarrow>
        Mem.loadv chk mem (Vlong (eval_snd_op_u64 (SOReg src) rs + scast (scast b_off)))\<noteq> None \<Longrightarrow>
        scast x_off = scast (scast x_off) \<Longrightarrow>
-       Vlong (rs' (BR dst)) = reg' (IR (bpf_to_x64_reg dst))"
+       Vlong (rs' dst) = reg' (IR (bpf_to_x64_reg dst))"
   apply (unfold exec_instr_def step)
   apply(cases xins)
   apply simp_all
   apply (unfold eval_load_def Let_def cast_lemma5, simp_all)
 apply (simp add: exec_load_def)
   apply (simp add: exec_load_def eval_addrmode64_def add64_def nextinstr_nf_def nextinstr_def)
-  apply (cases "loadv chk mem (Vlong (rs (BR src) + scast x_off))")
+  apply (cases "loadv chk mem (Vlong (rs src + scast x_off))")
    apply simp
-  apply (cases "loadv chk mem (Vlong (rs (BR src) + scast (scast x_off)))")
+  apply (cases "loadv chk mem (Vlong (rs src + scast (scast x_off)))")
   apply simp_all
   using cast_lemma5  load_subgoal_aux2_1
 *)
@@ -271,20 +271,20 @@ lemma load_subgoal_rr_aux2:
        a3:"ri = (bpf_to_x64_reg src)" and
        a4:"reg (IR rd) = Vlong n1" and
        a5:"reg (IR ri) = Vlong n2" and
-       a6:"n1 = rs (BR dst)" and
-       a7:"n2 = rs (BR src)" and
+       a6:"n1 = rs dst" and
+       a7:"n2 = rs dst" and
        a8:"x_off = ucast b_off " and
-       a9:"(BPF_OK rs' mem' ss  is_v1 cur_cu remain_cu) = step  bins rs mem ss is_v1 cur_cu remain_cu" and
+       a9:"(BPF_OK pc rs' mem' ss' is_v1 (cur_cu+1) remain_cu) = step fuel bins rs mem ss is_v1 cur_cu remain_cu" and
        a10:"Next reg' m' = exec_instr xins sz reg m" and
        a11:"m = mem" 
-       shows "Vlong (rs' (BR dst)) = reg' (IR (bpf_to_x64_reg dst))"
+       shows "Vlong (rs' dst) = reg' (IR (bpf_to_x64_reg dst))"
 proof-
   let ?t = "Addrmode (Some (bpf_to_x64_reg src)) None x_off"
   have "xins = Pmov_mr ?t rd chk" using Orderings.ord.ord_less_eq_trans Extraction.exE_realizer a0 apply simp
     using a1 a3 by fastforce
   let ?x = "eval_snd_op_u64 (SOReg src) rs + scast b_off"
   let ?tmp = "Mem.loadv chk mem (Vlong ?x)"
-  have b0:"step  bins rs mem ss is_v1 cur_cu remain_cu = (BPF_OK rs' mem' ss  is_v1 cur_cu remain_cu) \<longrightarrow> ?tmp \<noteq> None" 
+  have b0:"step fuel bins rs mem ss is_v1 cur_cu remain_cu = (BPF_OK pc rs' mem' ss' is_v1 (cur_cu+1) remain_cu) \<longrightarrow> ?tmp \<noteq> None" 
     using load_subgoal_aux2_2 using a0 a11 by blast
   have b1:"?tmp \<noteq> None" using b0 a9 by simp
   have b2:"Next reg' m' = exec_load sz chk m ?t reg (IR (bpf_to_x64_reg dst))" using exec_instr_def a1 apply (cases "xins") 
@@ -292,9 +292,9 @@ proof-
   have b3:"Next reg' m' = (case loadv chk m (eval_addrmode64 (?t) reg) 
            of None \<Rightarrow> Stuck | Some (v::val) \<Rightarrow> Next (nextinstr_nf sz (reg(IR (bpf_to_x64_reg dst) := v))) m) "
     using exec_load_def by (simp add: b2)
-  have b4:"Next reg' m' = (case loadv chk m (Vlong (rs (BR src) + scast x_off)) of None \<Rightarrow> Stuck
+  have b4:"Next reg' m' = (case loadv chk m (Vlong (rs src + scast x_off)) of None \<Rightarrow> Stuck
         | Some (v::val) \<Rightarrow> Next (nextinstr_nf sz (reg(IR (bpf_to_x64_reg dst) := v))) m)"
-    using eval_addrmode64_def b3 add64_def nextinstr_nf_def using a3 a5 a7 by force
+    using eval_addrmode64_def b3 add64_def nextinstr_nf_def using a3 a5 a7 sorry
   have b5:"Next reg' m' = Next (nextinstr_nf sz (reg(IR (bpf_to_x64_reg dst) := Option.the(?tmp)))) m" using b4 b1 apply (cases "bins")
     apply simp_all using a0  apply simp_all using a8 option.sel sorry
   have b6:" reg'(IR (bpf_to_x64_reg dst)) = Option.the(?tmp)" using nextinstr_nf_def nextinstr_def b5 by simp
@@ -305,14 +305,14 @@ proof-
   have " \<exists> x y. eval_load chk dst src b_off rs mem \<noteq> None \<longrightarrow> ?tmp = Some (Vlong x) \<or> ?tmp = Some (Vint y) " using c1_1 eval_load_def impI *)
 (*
   fix v1 assume "?tmp = Some(Vlong v1)" 
-  have c1_1:"(Option.the(?rss') (BR dst)) = v1" using a0 a9 the_def eval_load_def Let_def 
+  have c1_1:"(Option.the(?rss') dst) = v1" using a0 a9 the_def eval_load_def Let_def 
     using \<open>loadv (chk) (mem) (Vlong (eval_snd_op_u64 (SOReg (src)) (rs) + scast (b_off))) = Some (Vlong (v1))\<close> by force
   fix v2 assume "?tmp = Some(Vint v2)" 
-  have c1_2:"(Option.the(?rss') (BR dst)) = ucast v2" using a0 a9 the_def eval_load_def Let_def 
+  have c1_2:"(Option.the(?rss') dst) = ucast v2" using a0 a9 the_def eval_load_def Let_def 
     using \<open>loadv (chk) (mem) (Vlong (eval_snd_op_u64 (SOReg (src)) (rs) + scast (b_off))) = Some (Vint (v2))\<close> by force
   fix v3 assume "?tmp = None" 
  *)
-  have c1:"Vlong ((Option.the(?rss') (BR dst))) = Option.the(?tmp)" (*using a0 a9 the_def eval_load_def Let_def c0 cast_lemma6*)
+  have c1:"Vlong ((Option.the(?rss') dst)) = Option.the(?tmp)" (*using a0 a9 the_def eval_load_def Let_def c0 cast_lemma6*)
   proof (cases ?tmp)
     case None
     have d1:"eval_load chk dst src b_off rs mem = None" using eval_load_def 
@@ -346,10 +346,10 @@ proof-
            then show ?thesis using c0 d1 by simp
        qed
      qed
-  have c2:" (BPF_OK rs' mem' ss  is_v1 cur_cu remain_cu) = (BPF_OK ((Option.the(?rss'))#BPC <-- (1+ (Option.the(?rss') BPC))) mem ss  is_v1 cur_cu remain_cu) " 
+  have c2:" (BPF_OK pc rs' mem' ss is_v1 (cur_cu+1) remain_cu) = (BPF_OK ((Option.the(?rss'))#BPC <-- (1+ (Option.the(?rss') BPC))) mem ss  is_v1 cur_cu remain_cu) " 
     using c0 Let_def a9 a0 by auto
-  have c3:"Option.the(?rss')(BR dst) = rs' (BR dst)" using the_def c2 by simp
-  have c4:"Vlong (rs' (BR dst)) = Option.the(?tmp)" using c3 c1 by simp
+  have c3:"Option.the(?rss')dst = rs' dst" using the_def c2 by simp
+  have c4:"Vlong (rs' dst) = Option.the(?tmp)" using c3 c1 by simp
   thus ?thesis using c4 b6 by simp
 qed
 
@@ -379,93 +379,49 @@ lemma loadq_subgoal_rr_aux3:
         shows " \<forall> r \<noteq> dst. reg' (IR (bpf_to_x64_reg r)) = reg (IR (bpf_to_x64_reg r))"
  using cast_lemma6 a0 by (metis a1 bpf_to_x64_reg_corr load_subgoal_rr_aux3_1)
 
-lemma loadq_subgoal_rr_aux4:"bins = BPF_LDX chk dst src b_off \<Longrightarrow> (BPF_OK rs' m' ss'  is_v1 cur_cu remain_cu) = step  bins rs m ss is_v1 cur_cu remain_cu \<Longrightarrow>
-       \<forall> r \<noteq> dst. rs' (BR r) = rs (BR r)"
+lemma loadq_subgoal_rr_aux4:"bins = BPF_LDX chk dst src b_off \<Longrightarrow> (BPF_OK pc rs' m' ss' is_v1 (cur_cu+1) remain_cu) = step fuel bins rs m ss is_v1 cur_cu remain_cu \<Longrightarrow>
+       \<forall> r \<noteq> dst. rs' r = rs r"
   apply(cases "bins",simp_all)
   apply(unfold eval_load_def,simp)
-  apply(cases "loadv chk m (Vlong (rs (BR src) + scast b_off))" ,simp_all)
+  apply(cases "loadv chk m (Vlong (rs src + scast b_off))" ,simp_all)
   subgoal for a apply(cases a)
   by simp_all
   done
 
-
-
 lemma loadq_subgoal_rr_generic:
   assumes a0:"bins = BPF_LDX chk dst src b_off" and
        a1:"per_jit_load_reg64 dst src chk b_off = Some bl" and
-       a2:"list_in_list bl pc l_bin" and
-       a3:"x64_decode pc l_bin = Some (length l_bin, xins)" and
-       a4:"(BPF_OK rs' mem' ss'  is_v1 cur_cu remain_cu) = step  bins rs mem ss is_v1 cur_cu remain_cu" and
-       a5:"Next reg' m'  = exec_instr xins sz reg m" and
-       a6:"(\<forall> r. Vlong (rs (BR r)) = reg (IR (bpf_to_x64_reg r)))" and
+       a2:"list_in_list bl (unat pc) l_bin" and
+       a3:"x64_decode (unat pc) l_bin = Some (length l_bin, xins)" and
+       a4:"(BPF_OK pc rs' mem' ss' is_v1 (cur_cu+1) remain_cu) = step fuel bins rs mem ss is_v1 cur_cu remain_cu" and
+       a5:"Next reg' m' = exec_instr xins sz reg m" and
+       a6:"(\<forall> r. Vlong (rs r) = reg (IR (bpf_to_x64_reg r)))" and
        a7:"m = mem"
-  shows "(\<forall> r. Vlong (rs' (BR r)) = reg' (IR (bpf_to_x64_reg r)))"
+  shows "(\<forall> r. Vlong (rs' r) = reg' (IR (bpf_to_x64_reg r)))"
 proof -
   have b0:"xins = Pmov_mr (Addrmode (Some (bpf_to_x64_reg src)) None (ucast (b_off))) (bpf_to_x64_reg dst) chk" using x64_encode_decode_consistency per_jit_load_reg64_def a1 a2 a3 by fastforce
-    moreover have b1:"Vlong (rs (BR dst)) = reg (IR (bpf_to_x64_reg dst))" using a6 spec by simp
-    moreover have b2:"Vlong (rs (BR src)) = reg (IR (bpf_to_x64_reg src))" using a6 spec by simp
-    hence b3:"Vlong (rs' (BR dst)) = reg' (IR (bpf_to_x64_reg dst))" using load_subgoal_rr_aux2 b0 b1 b2 a0 a1 a2 a3 a4 a5 a6 a7 sorry
+    moreover have b1:"Vlong (rs dst) = reg (IR (bpf_to_x64_reg dst))" using a6 spec by simp
+    moreover have b2:"Vlong (rs src) = reg (IR (bpf_to_x64_reg src))" using a6 spec by simp
+    hence b3:"Vlong (rs' dst) = reg' (IR (bpf_to_x64_reg dst))" using load_subgoal_rr_aux2 b0 b1 b2 a0 a1 a2 a3 a4 a5 a6 a7 sorry
     have b4:"\<forall> r \<noteq> dst. reg'(IR (bpf_to_x64_reg r)) = reg (IR (bpf_to_x64_reg r))" using b0 a5 loadq_subgoal_rr_aux3 by blast
-    have b5:"\<forall> r \<noteq> dst. Vlong (rs'(BR r)) = Vlong (rs (BR r))" using a0 a4 loadq_subgoal_rr_aux4 by blast
-    have b6:"\<forall> r \<noteq> dst. Vlong (rs (BR r)) = reg (IR (bpf_to_x64_reg r))" using a6 by blast
-    have b7:"(\<forall> r \<noteq> dst. Vlong (rs' (BR r)) = reg' (IR (bpf_to_x64_reg r)))" by(simp add:b4 b5 b6) 
+    have b5:"\<forall> r \<noteq> dst. Vlong (rs' r) = Vlong (rs r)" using a0 a4 loadq_subgoal_rr_aux4 by blast
+    have b6:"\<forall> r \<noteq> dst. Vlong (rs r) = reg (IR (bpf_to_x64_reg r))" using a6 by blast
+    have b7:"(\<forall> r \<noteq> dst. Vlong (rs' r) = reg' (IR (bpf_to_x64_reg r)))" by(simp add:b4 b5 b6) 
     thus ?thesis using b3 by fastforce
   qed
-
-(*lemma store_subgoal_aux1:
-      "bins = BPF_ST chk dst (SOReg src) (b_off::i16) \<Longrightarrow>
-       xins = Pmov_rm ri (Addrmode (Some rd) None (x_off::u32)) chk \<Longrightarrow>
-       rd = (bpf_to_x64_reg dst)\<Longrightarrow>
-       ri = (bpf_to_x64_reg src) \<Longrightarrow>
-       reg (IR rd) = Vlong n1 \<Longrightarrow>
-       reg (IR ri) = Vlong n2 \<Longrightarrow>
-       n1  = rs (BR dst) \<Longrightarrow>
-       n2  = rs (BR src) \<Longrightarrow>
-       (BPF_OK rs' mem' ss'  is_v1 cur_cu remain_cu) = step  bins rs mem ss is_v1 cur_cu remain_cu \<Longrightarrow>
-       Next reg' m'  = exec_instr xins sz reg m \<Longrightarrow> 
-       m = mem \<Longrightarrow>
-       scast x_off = scast (scast x_off) \<Longrightarrow>
-       m' = mem'"
-  apply (unfold exec_instr_def step)
-  apply(cases xins)
-  apply simp_all
-  apply (unfold eval_store_def Let_def cast_lemma5, simp_all)
-  apply (simp add: exec_store_def eval_addrmode64_def add64_def nextinstr_nf_def nextinstr_def)
-  
-
-lemma store_subgoal_aux1:
-      "bins = BPF_ST chk dst (SOReg src) (b_off::i16) \<Longrightarrow>
-       xins = Pmov_rm ri (Addrmode (Some rd) None (x_off::u32)) chk \<Longrightarrow>
-       rd = (bpf_to_x64_reg dst)\<Longrightarrow>
-       ri = (bpf_to_x64_reg src) \<Longrightarrow>
-       reg (IR rd) = Vlong n1 \<Longrightarrow>
-       reg (IR ri) = Vlong n2 \<Longrightarrow>
-       n1  = rs (BR dst) \<Longrightarrow>
-       n2  = rs (BR src) \<Longrightarrow>
-       (BPF_OK rs' mem' ss'  is_v1 cur_cu remain_cu) = step  bins rs mem ss is_v1 cur_cu remain_cu \<Longrightarrow>
-       Next reg' m'  = exec_instr xins sz reg m \<Longrightarrow> 
-       m = mem \<Longrightarrow>
-       scast x_off = scast (scast x_off) \<Longrightarrow>
-      Vlong (rs' (BR dst)) = reg' (IR (bpf_to_x64_reg dst))"
-  apply (unfold exec_instr_def step)
-  apply(cases xins)
-  apply simp_all
-  apply (unfold eval_store_def Let_def cast_lemma5, simp_all)
-  apply (simp add: exec_store_def eval_addrmode64_def add64_def nextinstr_nf_def nextinstr_def)
-*) 
 
 lemma subq_subgoal_rr_aux1:
      "bins = BPF_ALU64 BPF_SUB dst (SOReg src) \<Longrightarrow>
      xins = Psubq_rr rd ri \<Longrightarrow>
-     (BPF_OK rs' m' ss'  is_v1 cur_cu remain_cu) = step  bins rs m ss is_v1 cur_cu remain_cu \<Longrightarrow>
+     (BPF_OK pc rs' m' ss' is_v1 (cur_cu+1) remain_cu) = step fuel bins rs m ss is_v1 cur_cu remain_cu \<Longrightarrow>
      Next reg' m'  = exec_instr xins sz reg m \<Longrightarrow>
      rd = (bpf_to_x64_reg dst) \<Longrightarrow>
      ri = (bpf_to_x64_reg src) \<Longrightarrow>
      reg (IR rd) = Vlong n1 \<Longrightarrow>
      reg (IR ri) = Vlong n2 \<Longrightarrow>
-     n1  = rs (BR dst) \<Longrightarrow>
-     n2  = rs (BR src) \<Longrightarrow> 
-     Vlong (rs' (BR dst)) = reg' (IR (bpf_to_x64_reg dst))"
+     n1  = rs dst \<Longrightarrow>
+     n2  = rs src \<Longrightarrow> 
+     Vlong (rs' dst) = reg' (IR (bpf_to_x64_reg dst))"
   apply (unfold exec_instr_def step)
   apply simp
   apply (unfold eval_alu64_def)
@@ -491,43 +447,41 @@ lemma subq_subgoal_rr_aux2:"xins = Psubq_rr (bpf_to_x64_reg dst) (bpf_to_x64_reg
   using bpf_to_x64_reg_corr subq_subgoal_rr_aux2_2 by metis
 
 
-lemma subq_subgoal_rr_aux3:"bins = BPF_ALU64 BPF_SUB dst (SOReg src) \<Longrightarrow> (BPF_OK rs' m' ss'  is_v1 cur_cu remain_cu) = step  bins rs m ss is_v1 cur_cu remain_cu \<Longrightarrow>
-       \<forall> r \<noteq> dst. rs' (BR r) = rs (BR r)"
+lemma subq_subgoal_rr_aux3:"bins = BPF_ALU64 BPF_SUB dst (SOReg src) \<Longrightarrow> (BPF_OK pc rs' m' ss' is_v1 (cur_cu+1) remain_cu) = step fuel bins rs m ss is_v1 cur_cu remain_cu \<Longrightarrow>
+       \<forall> r \<noteq> dst. rs' r = rs r"
   apply(cases "bins",simp_all)
   apply(unfold eval_alu64_def,simp)
   by (unfold eval_alu64_aux1_def, simp)
 
-
-
 lemma subq_subgoal_rr_generic:
   assumes a0:"bins = BPF_ALU64 BPF_SUB dst (SOReg src)" and
        a1:"per_jit_sub_reg64 dst src = Some bl" and
-       a2:"list_in_list bl pc l_bin" and
-       a3:"x64_decode pc l_bin = Some (length l_bin, xins)" and
-       a4:"(BPF_OK rs' m' ss'  is_v1 cur_cu remain_cu) = step  bins rs m ss is_v1 cur_cu remain_cu" and
+       a2:"list_in_list bl (unat pc) l_bin" and
+       a3:"x64_decode (unat pc) l_bin = Some (length l_bin, xins)" and
+       a4:"(BPF_OK pc rs' m' ss' is_v1 (cur_cu+1) remain_cu) = step fuel bins rs m ss is_v1 cur_cu remain_cu" and
        a5:"Next reg' m'  = exec_instr xins sz reg m" and
-       a6:"(\<forall> r. Vlong (rs (BR r)) = reg (IR (bpf_to_x64_reg r)))" 
-  shows "(\<forall> r. Vlong (rs' (BR r)) = reg' (IR (bpf_to_x64_reg r)))"
+       a6:"(\<forall> r. Vlong (rs r) = reg (IR (bpf_to_x64_reg r)))" 
+  shows "(\<forall> r. Vlong (rs' r) = reg' (IR (bpf_to_x64_reg r)))"
 proof -
   have b0:"xins = Psubq_rr (bpf_to_x64_reg dst) (bpf_to_x64_reg src)" using x64_encode_decode_consistency per_jit_sub_reg64_def a1 a2 a3 by fastforce
-    moreover have b1:"Vlong (rs (BR dst)) = reg (IR (bpf_to_x64_reg dst))" using a6 spec by simp
-    moreover have b2:"Vlong (rs (BR src)) = reg (IR (bpf_to_x64_reg src))" using a6 spec by simp
-    hence b3:"Vlong (rs' (BR dst)) = reg' (IR (bpf_to_x64_reg dst))" using subq_subgoal_rr_aux1 b0 b1 b2 a0 a4 a5 by force
+    moreover have b1:"Vlong (rs dst) = reg (IR (bpf_to_x64_reg dst))" using a6 spec by simp
+    moreover have b2:"Vlong (rs src) = reg (IR (bpf_to_x64_reg src))" using a6 spec by simp
+    hence b3:"Vlong (rs' dst) = reg' (IR (bpf_to_x64_reg dst))" using subq_subgoal_rr_aux1 b0 b1 b2 a0 a4 a5 by force
     have b4:"\<forall> r \<noteq> dst. reg'(IR (bpf_to_x64_reg r)) = reg (IR (bpf_to_x64_reg r))" using b0 a5 subq_subgoal_rr_aux2 by simp
-    have b5:"\<forall> r \<noteq> dst. Vlong (rs'(BR r)) = Vlong (rs (BR r))" using a0 a4 subq_subgoal_rr_aux3 by simp
-    have b6:"\<forall> r \<noteq> dst. Vlong (rs (BR r)) = reg (IR (bpf_to_x64_reg r))" using a6 by blast
-    have b7:"(\<forall> r \<noteq> dst. Vlong (rs' (BR r)) = reg' (IR (bpf_to_x64_reg r)))" by(simp add:b4 b5 b6) 
+    have b5:"\<forall> r \<noteq> dst. Vlong (rs' r) = Vlong (rs r)" using a0 a4 subq_subgoal_rr_aux3 by simp
+    have b6:"\<forall> r \<noteq> dst. Vlong (rs r) = reg (IR (bpf_to_x64_reg r))" using a6 by blast
+    have b7:"(\<forall> r \<noteq> dst. Vlong (rs' r) = reg' (IR (bpf_to_x64_reg r)))" by(simp add:b4 b5 b6) 
     thus ?thesis using b3 by fastforce
   qed
 
-lemma ja_subgoal_aux1:
+ (*Vlong (rs (BPC)) = reg PC \<Longrightarrow>*)
+(*lemma ja_subgoal_aux1:
       "bins = BPF_JA off \<Longrightarrow>
        xins = Pjmp d \<Longrightarrow>
-       Vlong (rs (BPC)) = reg PC \<Longrightarrow>
-       (BPF_OK rs' m' ss'  is_v1 cur_cu remain_cu) = step  bins rs m ss is_v1 cur_cu remain_cu \<Longrightarrow>
-       Next reg' m'  = exec_instr xins sz reg m \<Longrightarrow> 
+       (BPF_OK pc rs' m' ss' is_v1 (cur_cu+1) remain_cu) = step fuel bins rs m ss is_v1 cur_cu remain_cu \<Longrightarrow>
+       Next reg' m' = exec_instr xins sz reg m \<Longrightarrow> 
        d = ucast(off::i16)\<Longrightarrow>
-      Vlong (rs' (BPC))= reg' PC"
+       pc = reg' PC"
   apply (unfold exec_instr_def step)
   apply simp
   apply (unfold eval_pc_def nextinstr_def add64_def)
@@ -535,7 +489,7 @@ lemma ja_subgoal_aux1:
   apply(erule conjE)+
   apply(cases "reg RIP", simp_all)
   using cast_lemma4 by auto
-
+*)
 
 lemma ja_subgoal_aux2:"xins = Pjmp d \<Longrightarrow> Next reg' m' = exec_instr xins sz reg m \<Longrightarrow>
        \<forall> r. reg' (IR (bpf_to_x64_reg r)) = reg (IR (bpf_to_x64_reg r))"
@@ -543,43 +497,41 @@ lemma ja_subgoal_aux2:"xins = Pjmp d \<Longrightarrow> Next reg' m' = exec_instr
   apply(unfold nextinstr_nf_def nextinstr_def add64_def) 
   by auto
 
-lemma ja_subgoal_aux3:"bins = BPF_JA off \<Longrightarrow> (BPF_OK rs' m' ss'  is_v1 cur_cu remain_cu) = step  bins rs m ss is_v1 cur_cu remain_cu \<Longrightarrow>
-       \<forall> r. rs' (BR r) = rs (BR r)"
+lemma ja_subgoal_aux3:"bins = BPF_JA off \<Longrightarrow> (BPF_OK pc rs' m' ss' is_v1 cur_cu remain_cu) = step fuel bins rs m ss is_v1 cur_cu remain_cu \<Longrightarrow>
+       \<forall> r. rs' r = rs r"
   by(cases "bins",simp_all)
 
 lemma ja_subgoal_generic:
   assumes a0:"bins = BPF_JA off" and
-       a1:" per_jit_ja (ucast off) = Some bl" and
-       a2:"list_in_list bl pc l_bin" and
-       a3:"x64_decode pc l_bin = Some (length l_bin, xins)" and
-       a4:"(BPF_OK rs' m' ss'  is_v1 cur_cu remain_cu) = step  bins rs m ss is_v1 cur_cu remain_cu" and
+       a1:"per_jit_ja (ucast off) = Some bl" and
+       a2:"list_in_list bl (unat pc) l_bin" and
+       a3:"x64_decode (unat pc) l_bin = Some (length l_bin, xins)" and
+       a4:"(BPF_OK pc rs' m' ss' is_v1 (cur_cu+1) remain_cu) = step fuel bins rs m ss is_v1 cur_cu remain_cu" and
        a5:"Next reg' m' = exec_instr xins sz reg m" and
-       a6:"(\<forall> r. Vlong (rs (BR r)) = reg (IR (bpf_to_x64_reg r))) \<and> Vlong (rs (BPC)) = reg PC" 
-  shows "(\<forall> r. Vlong (rs' (BR r)) = reg' (IR (bpf_to_x64_reg r))) \<and> Vlong (rs' (BPC))= reg' PC"
+       a6:"(\<forall> r. Vlong (rs r) = reg (IR (bpf_to_x64_reg r)))" 
+  shows "(\<forall> r. Vlong (rs' r) = reg' (IR (bpf_to_x64_reg r)))"
 proof -
-  have b0:"xins = Pjmp (ucast off)" using x64_encode_decode_consistency per_jit_ja_def a1 a2 a3 by fastforce
-  moreover have b1:"Vlong (rs (BPC)) = reg PC" using a6 by simp
-  moreover have b2:"(\<forall> r. Vlong (rs (BR r)) = reg (IR (bpf_to_x64_reg r)))" using a6 by simp
-    hence b3:"Vlong (rs' (BPC))= reg' PC" using ja_subgoal_aux1 b0 b1 a0 a4 a5 by force
-    have b4:"\<forall> r. reg'(IR (bpf_to_x64_reg r)) = reg (IR (bpf_to_x64_reg r))" using b0 b1 a5 ja_subgoal_aux2 by simp
-    have b5:"\<forall> r. Vlong (rs'(BR r)) = Vlong (rs (BR r))" using a0 a4 ja_subgoal_aux3 by simp
-    have b6:"\<forall> r. Vlong (rs (BR r)) = reg (IR (bpf_to_x64_reg r))" using a6 by blast
-    have b7:"(\<forall> r. Vlong (rs' (BR r)) = reg' (IR (bpf_to_x64_reg r)))" by(simp add:b4 b5 b6) 
-    thus ?thesis using b3 by fastforce
+  have b0:"xins = Pjmp (ucast off)" using x64_encode_decode_consistency per_jit_ja_def a1 a2 a3 sorry
+  moreover have b2:"(\<forall> r. Vlong (rs r) = reg (IR (bpf_to_x64_reg r)))" using a6 by simp
+    have b4:"\<forall> r. reg'(IR (bpf_to_x64_reg r)) = reg (IR (bpf_to_x64_reg r))" using b0 a5 ja_subgoal_aux2 by simp
+    have b5:"\<forall> r. Vlong (rs' r) = Vlong (rs r)" using a0 a4 ja_subgoal_aux3 by simp
+    have b6:"\<forall> r. Vlong (rs r) = reg (IR (bpf_to_x64_reg r))" using a6 by blast
+    have b7:"(\<forall> r. Vlong (rs' r) = reg' (IR (bpf_to_x64_reg r)))" by(simp add:b4 b5 b6) 
+    thus ?thesis using b7 by fastforce
   qed
 
 
 lemma subl_subgoal_ri:
       "bins = BPF_ALU BPF_SUB dst (SOImm src) \<Longrightarrow>
        xins = Psubl_ri rd imm \<Longrightarrow>
-       (BPF_OK rs' m' ss'  is_v1 cur_cu remain_cu) = step  bins rs m ss is_v1 cur_cu remain_cu \<Longrightarrow>
+       (BPF_OK pc rs' m' ss' is_v1 (cur_cu+1) remain_cu) = step fuel bins rs m ss is_v1 cur_cu remain_cu \<Longrightarrow>
        Next reg' m'  = exec_instr xins sz reg m \<Longrightarrow> 
-       corr_registers dst rd \<Longrightarrow>
+       rd = bpf_to_x64_reg dst \<Longrightarrow>
        imm = ucast (src) \<Longrightarrow>
        reg (IR rd) = Vint n1 \<Longrightarrow>
-       ucast n1  = rs (BR dst) \<Longrightarrow>
+       ucast n1  = rs dst \<Longrightarrow>
        reg' (IR rd) = Vint n3 \<Longrightarrow>
-       ucast n3 = rs'(BR dst)"
+       ucast n3 = rs'dst"
   apply (unfold exec_instr_def step)
   apply simp
   apply (unfold eval_alu32_def)
@@ -592,8 +544,8 @@ lemma subl_subgoal_ri:
   apply simp
   apply (unfold add64_def)
   apply (erule conjE)
-  apply (cases "is_v1 cur_cu remain_cu", simp_all)
-  apply (cases "is_v1 cur_cu remain_cu", simp_all)
+  apply (cases "is_v1", simp_all)
+  apply (cases "is_v1", simp_all)
   using cast_lemma2 
   sorry
 
@@ -601,17 +553,17 @@ lemma subl_subgoal_ri:
 lemma movq_subgoal_rr:
       "bins = BPF_ALU64 BPF_MOV dst (SOReg src) \<Longrightarrow>
        xins = Pmovq_rr rd ri \<Longrightarrow>
-       (BPF_OK rs' m' ss'  is_v1 cur_cu remain_cu) = step  bins rs m ss is_v1 cur_cu remain_cu \<Longrightarrow>
+       (BPF_OK pc rs' m' ss' is_v1 (cur_cu+1) remain_cu) = step fuel bins rs m ss is_v1 cur_cu remain_cu \<Longrightarrow>
        Next reg' m'  = exec_instr xins sz reg m \<Longrightarrow> 
-       corr_registers dst rd \<Longrightarrow>
-       corr_registers src ri \<Longrightarrow>
+       rd = bpf_to_x64_reg dst \<Longrightarrow>
+       ri = bpf_to_x64_reg src \<Longrightarrow>
        reg (IR rd) = Vlong n1 \<Longrightarrow>
        reg (IR ri) = Vlong n2 \<Longrightarrow>
-       n1  = rs (BR dst) \<Longrightarrow>
-       n2  = rs (BR src) \<Longrightarrow>
+       n1  = rs dst \<Longrightarrow>
+       n2  = rs src \<Longrightarrow>
        reg' (IR rd) = Vlong n3 \<Longrightarrow>
-       ucast n3 = rs'(BR dst)"
-(*memory_mapping bstate = m' \<and> (reg' (IR rd)) = Vlong (rs'(BR dst))"*)
+       ucast n3 = rs'dst"
+(*memory_mapping bstate = m' \<and> (reg' (IR rd)) = Vlong (rs'dst)"*)
   apply (unfold exec_instr_def step)
   apply simp
   apply (unfold eval_alu64_def)
@@ -623,21 +575,21 @@ lemma movq_subgoal_rr:
 lemma movq_subgoal_ri:
       "bins = BPF_ALU64 BPF_MOV dst (SOImm src) \<Longrightarrow>
        xins = Pmovq_ri rd imm \<Longrightarrow>
-       (BPF_OK rs' m' ss'  is_v1 cur_cu remain_cu) = step  bins rs m ss is_v1 cur_cu remain_cu \<Longrightarrow>
+       (BPF_OK pc rs' m' ss' is_v1 (cur_cu+1) remain_cu) = step fuel bins rs m ss is_v1 cur_cu remain_cu \<Longrightarrow>
        Next reg' m' = exec_instr xins sz reg m \<Longrightarrow> 
-       corr_registers dst rd \<Longrightarrow>
+       rd = bpf_to_x64_reg dst \<Longrightarrow>
        imm = ucast (src) \<Longrightarrow>
        reg (IR rd) = Vlong n1 \<Longrightarrow>
-       ucast n1  = rs (BR dst) \<Longrightarrow>
+       ucast n1  = rs dst \<Longrightarrow>
        reg' (IR rd) = Vlong n3 \<Longrightarrow>
-       ucast n3 = rs'(BR dst)"
+       ucast n3 = rs'dst"
   apply (unfold exec_instr_def step)
   apply simp
   apply (unfold eval_alu64_def)
   apply (cases BPF_MOV, simp_all)
   apply (unfold nextinstr_def)
   apply (erule conjE)
-  apply (metis (no_types, lifting) option.case_eq_if option.discI option.sel rbpf_state.select_convs(2))
+  try
   apply(unfold eval_alu64_aux1_def add64_def) 
   by simp
 
