theory/rBPFDecoder.thy
@@ -296,7 +296,42 @@ definition bpf_find_instr :: "nat \<Rightarrow> u8 list \<Rightarrow> bpf_instru
     )
 )"
 
+definition getNextPC::"nat \<Rightarrow> u8 list \<Rightarrow> nat" where
+"getNextPC pc l = (
+  let npc= pc*INSN_SIZE in
+    let off_v = u16_of_u8_list [l!(npc+2), l!(npc+3)] in
+      if unat (Option.the off_v) = 0 then 1+pc
+      else unat (Option.the off_v) + pc
+)"
+
+fun bpf_find_prog_aux :: "nat \<Rightarrow> nat \<Rightarrow> u8 list \<Rightarrow> bpf_instruction option list " where
+"bpf_find_prog_aux 0 _ _ = [None] " |
+"bpf_find_prog_aux (Suc fuel) pc l = (if (pc+1)*INSN_SIZE \<le> length l then 
+  (let ins' = bpf_find_instr pc l in 
+              case ins' of None \<Rightarrow> [None] |
+                           Some v \<Rightarrow> let pc' = getNextPC pc l in
+        [Some v] @ bpf_find_prog_aux fuel pc' l) else [None])"
+
+definition bpf_find_prog::"nat \<Rightarrow> nat \<Rightarrow> u8 list \<Rightarrow> bpf_instruction list option" where
+"bpf_find_prog fuel pc l  = (let l' = bpf_find_prog_aux fuel pc l in 
+                              if length l' = 1 then None else Some (map Option.the (butlast l')))"
+
+
+value "length [None]"
+
+value "map Option.the ([Some (BPF_ADD_STK 67305985), Some (BPF_ADD_STK 67305985)])"
+
+value "butlast (bpf_find_prog_aux 3 0 [0x07::u8,0x0B,0x00,0x00,0x01,0x02,0x03,0x04]) "
 
 value "bpf_find_instr 0 [0x07::u8,0x0B,0x00,0x00,0x01,0x02,0x03,0x04] "
+
+value "bpf_find_prog_aux 3 0 [0x07::u8,0x0B,0x00,0x00,0x01,0x02,0x03,0x04] "
+
+value "bpf_find_prog 3 0 [0x07::u8,0x0B,0x00,0x00,0x01,0x02,0x03,0x04,
+  0x07::u8,0x0B,0x00,0x00,0x01,0x02,0x03,0x04] "
+
+value "getNextPC 0 [0x07::u8,0x0B,0x00,0x00,0x01,0x02,0x03,0x04] "
+
+
 
 end
