theory/x64DecodeProof.thy
@@ -57,7 +57,8 @@ lemma x64_encode_decode_consistency:
   "list_in_list l_bin pc l \<Longrightarrow> Some l_bin = x64_encode ins \<Longrightarrow>
     x64_decode pc l = Some (length l_bin, ins)"
   sorry
- (* apply (cases ins; simp_all)
+ (* 
+ apply (cases ins; simp_all)
 
   subgoal for dst src
   \<comment> \<open> Pmovl_rr \<close> 
@@ -1166,7 +1167,7 @@ e
     \<comment> \<open> Pnop \<close>
     apply(unfold Let_def x64_decode_def; simp)
     done
-  done
-*)
+  done*)
+
 declare if_split_asm [split del]
 end
